src/Lib/BCT/Vst.v
@@ -34,7 +34,7 @@ Definition ber_check_tags_spec : ident * funspec :=
          td_p : val, td : TYPE_descriptor, 
          tags_p : val,
          opt_ctx_p : val,
-         b : block, i : ptrofs, ptr : list Z,
+         b : block, i : ptrofs, ptr : list int,
          res_p : val,
          size : Z, tag_mode : Z, last_tag_form : Z,
          last_length_p : val,
@@ -47,12 +47,12 @@ Definition ber_check_tags_spec : ident * funspec :=
       PROP (tag_mode = 0;
             last_tag_form = 0;
             0 < len ptr <= Ptrofs.max_unsigned;
-            (Znth 0 ptr) & 32 = 0;
+            (Znth 0 ptr & Int.repr 32 = 0)%int;
             nullval = opt_ctx_p;
             nullval = opt_tlv_form_p;
             1 = len (tags td);
             0 <= Ptrofs.unsigned i + len ptr <= Ptrofs.max_unsigned;
-            Forall (fun x => 0 <= x <= Byte.max_unsigned) ptr;
+            Forall (fun x => 0 <= Int.unsigned x <= Byte.max_unsigned) ptr;
             0 <= size <= Int.max_unsigned)
       PARAMS (res_p; opt_codec_ctx_p; td_p; opt_ctx_p; (Vptr b i); 
                 Vint (Int.repr size);
@@ -60,7 +60,7 @@ Definition ber_check_tags_spec : ident * funspec :=
                   last_length_p; opt_tlv_form_p)
       GLOBALS ((* (fun _ : ident => Vint 0%int) *))
       SEP (data_at Tsh (tarray tuchar (len ptr)) 
-                   (map Vint (map Int.repr ptr)) (Vptr b i);
+                   (map Vint ptr) (Vptr b i);
            field_at Tsh (Tstruct _asn_TYPE_descriptor_s noattr) 
                          [StructField _tags] 
                          tags_p td_p;
@@ -77,7 +77,7 @@ Definition ber_check_tags_spec : ident * funspec :=
       PROP ()
       LOCAL ()
       SEP (data_at Tsh (tarray tuchar (len ptr)) 
-                   (map Vint (map Int.repr ptr)) (Vptr b i);
+                   (map Vint ptr) (Vptr b i);
            field_at Tsh (Tstruct _asn_TYPE_descriptor_s noattr) 
                          [StructField _tags] 
                          tags_p td_p;
@@ -88,9 +88,9 @@ Definition ber_check_tags_spec : ident * funspec :=
                    (map Vint (map Int.repr (tags td))) tags_p;
            data_at Tsh (Tstruct _asn_codec_ctx_s noattr) 
                   (Vint (Int.repr (max_stack_size))) opt_codec_ctx_p;
-           match ber_check_tags_primitive (map Int.repr ptr)
+           match ber_check_tags_primitive ptr
                                        td max_stack_size
-                                       size (sizeof tuint) Int.modulus with
+                                       size (sizeof tuint) Int.max_signed with
            | Some v => 
              data_at Tsh asn_dec_rval_s 
                      (mk_dec_rval 0 (snd v)) res_p *
@@ -123,18 +123,16 @@ Theorem ber_check_tags_correctness :
   semax_body Vprog Gprog
              (normalize_function f_ber_check_tags composites) 
              ber_check_tags_spec.
-Admitted.
-(*
-Proof.
+(* Proof.
   start_function.
   subst.
   repeat forward.
   forward_if (temp _t'1 Vzero).
   contradiction.
-  - (* forward.
-    entailer!. *) admit.
   - forward.
-    forward_call (opt_codec_ctx_p, max_stack_size).
+    entailer!.
+  - forward.
+    Time forward_call (opt_codec_ctx_p, max_stack_size).
       assert (-1 <= ASN__STACK_OVERFLOW_CHECK 0 max_stack_size <= 0) as A.
     { unfold ASN__STACK_OVERFLOW_CHECK.
       repeat break_if; lia. }
@@ -142,14 +140,14 @@ Proof.
                 (if eq_dec opt_codec_ctx_p nullval
                  then 0
                  else ASN__STACK_OVERFLOW_CHECK 0 max_stack_size) = 0].
-  + admit. (* forward_empty_while.
+  +  forward_empty_while.
   assert (opt_codec_ctx_p <> nullval) as ON.
   { break_if; try nia.
     eassumption. }
   rewrite_if_b. 
   forward_if True; try contradiction.
-  * (* forward.
-    entailer!. *) admit.
+  * forward.
+    entailer!. 
   * forward_if (temp _t'2 Vzero);
       try forward; try entailer!.
     forward_if_add_sep (data_at Tsh (Tstruct _asn_dec_rval_s noattr)
@@ -165,17 +163,17 @@ Proof.
          erewrite AS.
          auto. }
     erewrite N.
-    entailer!.  *)
-  + admit. (* forward.    
+    entailer!. 
+  + forward.    
     entailer!.
     apply repr_inj_signed.
-    repeat break_if; try rep_omega.
-    rep_omega.
-    eassumption. *)
+    repeat break_if; try rep_lia.
+    rep_lia.
+    eassumption. 
   + forward_if
       (temp _t'4 Vzero); try congruence.
-  -- admit. (* forward.
-     entailer!. *)
+  -- forward.
+     entailer!.
   -- forward.
      forward_if (temp _t'10 
                   ((force_val
@@ -185,10 +183,9 @@ Proof.
                        (Int.repr 0))
                     (eval_cast tuint tint (Vint (Int.repr (len (tags td))))))))
                    )); try discriminate.
-     --- admit. 
-         (* forward.
+     --- forward.
          forward.
-         entailer!. *) 
+         entailer!. 
      ---
        Arguments eq_dec : simpl never.
        forward_if True.
@@ -207,15 +204,10 @@ Proof.
        forward.
        forward_if True.
        forward.
-       admit. (* entailer!. *)
-    (*   match goal with
-       | [ _ : _ |-  semax _ (PROPx ?P (LOCALx ?Q (SEPx ?R))) ?C ?Post ] =>
-         replace Q with (gvars (fun x : ident => nullval) :: Q)
-        end. *)
-       (* assert_fail *)
+       entailer!.
        forward_call (false).
-       admit. (* entailer!. *)
-       admit. (* entailer!. *)
+       entailer!.
+       entailer!.
      (* MAIN LOOP *)       
      (* match goal with
        | [ _ : _ |-  semax _ (PROPx ?P (LOCALx ?Q (SEPx ?R))) ?C ?Post ] =>
@@ -229,7 +221,7 @@ Proof.
          let Q'' := remove_LOCAL _step Q' in *)
          forward_loop (
      EX z : Z,
-     let (tag_len, tlv_tag) := Exec.ber_fetch_tags (map Int.repr ptr)
+     let (tag_len, tlv_tag) := Exec.ber_fetch_tags ptr
                                                    size  in
      let (len_len, tlv_len) := Exec.ber_fetch_len (sublist 1 (len ptr) ptr) 0 0 
                                                   (size - tag_len) (sizeof tuint) Int.modulus in
@@ -244,7 +236,7 @@ Proof.
            tag_len <> 0 /\
            len_len <> -1 /\
            len_len <> 0 /\ 
-           tlv_tag = nth O (tags td) 0)
+           tlv_tag = (Int.repr (nth O (tags td) 0)))
      LOCAL (temp _t'10
               (force_val
                  (sem_cast tint tbool
@@ -305,9 +297,9 @@ Proof.
      if z =? 0 then (data_at_ Tsh tint v_tlv_len *
                      data_at_ Tsh tuint v_tlv_tag)
      else (data_at Tsh tint (Vint (Int.repr tlv_len)) v_tlv_len *
-                     data_at Tsh tuint (Vint (Int.repr tlv_tag)) v_tlv_tag);
+                     data_at Tsh tuint (Vint (tlv_tag)) v_tlv_tag);
      data_at Tsh (tarray tuchar (len ptr)) 
-             (map Vint (map Int.repr ptr)) (Vptr b i);
+             (map Vint ptr) (Vptr b i);
      field_at Tsh (Tstruct _asn_TYPE_descriptor_s noattr) (DOT _tags) tags_p td_p;
      field_at Tsh (Tstruct _asn_TYPE_descriptor_s noattr) (DOT _tags_count)
        (Vint (Int.repr (len (tags td)))) td_p;
@@ -317,7 +309,9 @@ Proof.
      data_at_ Tsh tint last_length_p))%assert
                       (* CONTINUE *)
                       continue:
-           (let (tag_len, tlv_tag) := Exec.ber_fetch_tags ptr size 0 (sizeof tuint) in
+           (let (tag_len, tlv_tag) := 
+                Exec.ber_fetch_tags ptr
+                                    size  in
        let (len_len, tlv_len) :=
          Exec.ber_fetch_len (sublist 1 (len ptr) ptr) 0 0 (size - tag_len) 
            (sizeof tuint) Int.modulus in
@@ -327,7 +321,7 @@ Proof.
            tag_len <> 0;
            len_len <> -1;
            len_len <> 0;
-           tlv_tag = nth O (tags td) 0)
+           tlv_tag = Int.repr (nth O (tags td) 0))
        LOCAL (temp _t'10
                 (force_val
                    (sem_cast tint tbool
@@ -375,15 +369,16 @@ Proof.
        data_at_ Tsh (Tstruct _asn_dec_rval_s noattr) v_rval__1;
        data_at_ Tsh (Tstruct _asn_dec_rval_s noattr) v_rval;
         data_at Tsh tint (Vint (Int.repr tlv_len)) v_tlv_len ;
-        data_at Tsh tuint (Vint (Int.repr tlv_tag)) v_tlv_tag;
-       data_at Tsh (tarray tuchar (len ptr)) (map Vint (map Int.repr ptr)) (Vptr b i);
+        data_at Tsh tuint (Vint (tlv_tag)) v_tlv_tag;
+       data_at Tsh (tarray tuchar (len ptr)) (map Vint ptr) (Vptr b i);
        field_at Tsh (Tstruct _asn_TYPE_descriptor_s noattr) (DOT _tags) tags_p td_p;
        field_at Tsh (Tstruct _asn_TYPE_descriptor_s noattr) (DOT _tags_count)
          (Vint (Int.repr (len (tags td)))) td_p;
        data_at Tsh (tarray tuint (len (tags td))) (map Vint (map Int.repr (tags td))) tags_p;
        data_at_ Tsh asn_dec_rval_s res_p; data_at_ Tsh tint last_length_p))
                              break: (
-     let (tag_len, tlv_tag) := Exec.ber_fetch_tags ptr size 0 (sizeof tuint) in
+     let (tag_len, tlv_tag) := Exec.ber_fetch_tags ptr
+                                                   size in
      let (len_len, tlv_len) := Exec.ber_fetch_len (sublist 1 (len ptr) ptr) 0 0 
                                                   (size - tag_len) (sizeof tuint) Int.modulus in
      PROP (0 < tag_len;
@@ -392,7 +387,7 @@ Proof.
            tag_len <> 0;
            len_len <> -1;
            len_len <> 0;
-           tlv_tag = nth O (tags td) 0)
+           tlv_tag = Int.repr (nth O (tags td) 0))
      LOCAL (temp _t'10
               (force_val
                  (sem_cast tint tbool
@@ -449,9 +444,9 @@ Proof.
      data_at_ Tsh (Tstruct _asn_dec_rval_s noattr) v_rval__1;
      data_at_ Tsh (Tstruct _asn_dec_rval_s noattr) v_rval;
      data_at Tsh tint (Vint (Int.repr tlv_len)) v_tlv_len;
-     data_at Tsh tuint (Vint (Int.repr tlv_tag)) v_tlv_tag;
+     data_at Tsh tuint (Vint (tlv_tag)) v_tlv_tag;
      data_at Tsh (tarray tuchar (len ptr)) 
-             (map Vint (map Int.repr ptr)) (Vptr b i);
+             (map Vint ptr) (Vptr b i);
      field_at Tsh (Tstruct _asn_TYPE_descriptor_s noattr) (DOT _tags) tags_p td_p;
      field_at Tsh (Tstruct _asn_TYPE_descriptor_s noattr) (DOT _tags_count)
        (Vint (Int.repr (len (tags td)))) td_p;
@@ -461,11 +456,11 @@ Proof.
      data_at_ Tsh tint last_length_p))
        end.
        +++ (* Pre -> LI *)
-        (* Exists 0.
+         Exists 0.
          repeat rewrite_if_b.
          repeat break_let.
          entailer!.
-         apply derives_refl. *) admit.
+         apply derives_refl. 
        +++ Intros z.
            repeat break_let.
            break_if.
@@ -475,18 +470,261 @@ Proof.
              forward.
            forward_if.
            2: (* LI -> break *) lia.
-           forward_call (b, i, ptr, size, v_tlv_tag). 
-           { repeat split; try rep_omega.
-             eassumption. }
-           assert (z0 = 65) as Z0 by admit.
-           replace (fst (Exec.ber_fetch_tags ptr size 0 (sizeof tuint)))
-             with z0. (* FIXME : forward switch doesn't work with complex terms *)
+           deadvars.
+           Time forward_call (b, i, ptr, size, v_tlv_tag). 
+           unfold Frame.
+            instantiate (1 := [emp]).
+            simpl.
+            admit.
+           { repeat split; try rep_lia.
+             all: admit. }
+           
+          
+
+
+
+
+               Require Import VST.floyd.proofauto.
+                Set Ltac Backtrace.
+                Ltac process_cases sign ::= 
+match goal with
+| |- semax _ _ (seq_of_labeled_statement 
+     match select_switch_case ?N (LScons (Some ?X) ?C ?SL)
+      with Some _ => _ | None => _ end) _ =>
+       let y := constr:(adjust_for_sign sign X) in let y := eval compute in y in 
+      rewrite (select_switch_case_signed y); 
+           [ | reflexivity | clear; compute; split; congruence];
+     let E := fresh "E" in let NE := fresh "NE" in 
+     destruct (zeq N (Int.unsigned (Int.repr y))) as [E|NE];
+      [ try ( rewrite if_true; [  | symmetry; apply E]);
+        unfold seq_of_labeled_statement at 1;
+        apply unsigned_eq_eq in E;
+        match sign with
+        | Signed => apply repr_inj_signed in E; try rep_lia
+        | Unsigned => apply repr_inj_unsigned in E;  try rep_lia
+        end;
+        try match type of E with ?a = _ => is_var a; subst a end;
+        repeat apply -> semax_skip_seq
+     | try (rewrite if_false by (contradict NE; symmetry; apply NE));
+        process_cases sign
+    ]
+| |- semax _ _ (seq_of_labeled_statement 
+     match select_switch_case ?N (LScons None ?C ?SL)
+      with Some _ => _ | None => _ end) _ =>
+      change (select_switch_case N (LScons None C SL))
+       with (select_switch_case N SL);
+        process_cases sign
+| |- semax _ _ (seq_of_labeled_statement 
+     match select_switch_case ?N LSnil
+      with Some _ => _ | None => _ end) _ =>
+      change (select_switch_case N LSnil)
+           with (@None labeled_statements);
+      cbv iota;
+      unfold seq_of_labeled_statement at 1;
+      repeat apply -> semax_skip_seq
+end.
+                Time match goal with
+                  | [ _ : _ |- semax _ ?Pre ?C ?Post ] =>
+               forward_if Pre                              
+             end.
+Ltac process_cases sign ::= 
+match goal with
+| |- semax _ _ (seq_of_labeled_statement 
+     match select_switch_case ?N (LScons (Some ?X) ?C ?SL)
+      with Some _ => _ | None => _ end) _ =>
+      let y := constr:(adjust_for_sign sign X) in 
+      let y := eval compute in y in 
+      rewrite (select_switch_case_signed y); 
+           [ | reflexivity | clear; compute; split; congruence];
+     let E := fresh "E" in let NE := fresh "NE" in 
+     destruct (zeq N (Int.unsigned (Int.repr y))) as [E|NE];
+      [ try ( rewrite if_true; [  | symmetry; apply E]);
+        unfold seq_of_labeled_statement at 1;
+        apply unsigned_eq_eq in E;
+         match sign with
+        | Signed =>  (apply repr_inj_signed in E; [ | rep_lia | rep_lia])
+        | Unsigned =>  (apply repr_inj_unsigned in E; [ | rep_lia | rep_lia])
+        end;
+        try match type of E with ?a = _ => is_var a; subst a end;
+        repeat apply -> semax_skip_seq 
+        | 
+        try (rewrite if_false by (contradict NE; symmetry; apply NE));
+        process_cases sign  
+    ] 
+
+| |- semax _ _ (seq_of_labeled_statement 
+     match select_switch_case ?N (LScons None ?C ?SL)
+      with Some _ => _ | None => _ end) _ =>
+      change (select_switch_case N (LScons None C SL))
+       with (select_switch_case N SL);
+      process_cases sign
+
+| |- semax _ _ (seq_of_labeled_statement 
+     match select_switch_case ?N LSnil
+      with Some _ => _ | None => _ end) _ =>
+      change (select_switch_case N LSnil)
+           with (@None labeled_statements);
+      cbv iota;
+      unfold seq_of_labeled_statement at 1;
+      repeat apply -> semax_skip_seq
+
+end. 
+
+
+             Time match goal with
+                  | [ _ : _ |- semax _ ?Pre ?C ?Post ] =>
+               forward_if Pre                              
+             end.
+             congruence.
+             process_cases Signed.
+             congruence.
+             process_cases Signed.
+             process_cases Signed.
+             change (select_switch_case (Int.unsigned (Int.repr 0))
+                                        (LScons None Sbreak LSnil))
+               with (select_switch_case (Int.unsigned (Int.repr 0)) LSnil).
+
+             change (select_switch_case (Int.unsigned (Int.repr 0)) LSnil)
+               with (@None labeled_statements);
+               cbv iota;
+               unfold seq_of_labeled_statement at 1;
+               repeat apply -> semax_skip_seq.
+             forward.
+               process_cases Signed.
+             
+apply repr_inj_signed in E; [ | try rep_lia | try rep_lia].
+           
+                     
+             Set Ltac Backtrace.
+             unfold MORE_COMMANDS.
+             unfold abbreviate.
+             
+             match goal with
+             | [ _ : _ |- semax _ ?Pre ?C ?Post ] =>
+               forward_switch Pre 
+                              
+             end.
+
+          (* FIXME : forward switch doesn't work with complex terms *)
            (* in VST 2.6 forward_switch needs change and can fail here *)
+           Require Import Forward.
+           Set Ltac Backtrace.
+
+           
+          
+           Ltac process_cases sign := 
+match goal with
+| |- semax _ _ (seq_of_labeled_statement 
+     match select_switch_case ?N (LScons (Some ?X) ?C ?SL)
+      with Some _ => _ | None => _ end) _ =>
+       let y := constr:(adjust_for_sign sign X) in let y := eval compute in y in 
+      rewrite (select_switch_case_signed y); 
+           [ | reflexivity | clear; compute; split; congruence];
+     let E := fresh "E" in let NE := fresh "NE" in 
+     destruct (zeq (Int.unsigned (Int.repr y)) N) as [E|NE];
+      [ unfold seq_of_labeled_statement at 1 ;
+        apply unsigned_eq_eq in E;
+        match sign with
+        | Signed => apply repr_inj_signed in E; [ | rep_omega | rep_omega]
+        | Unsigned => apply repr_inj_unsigned in E; [ | rep_omega | rep_omega]
+        end;
+        try match type of E with ?a = _ => is_var a; subst a end;
+        repeat apply -> semax_skip_seq
+     | process_cases sign
+    ]
+| |- semax _ _ (seq_of_labeled_statement 
+     match select_switch_case ?N (LScons None ?C ?SL)
+      with Some _ => _ | None => _ end) _ =>
+      change (select_switch_case N (LScons None C SL))
+       with (select_switch_case N SL);
+      process_cases sign
+| |- semax _ _ (seq_of_labeled_statement 
+     match select_switch_case ?N LSnil
+      with Some _ => _ | None => _ end) _ =>
+      change (select_switch_case N LSnil)
+           with (@None labeled_statements);
+      cbv iota;
+      unfold seq_of_labeled_statement at 1;
+      repeat apply -> semax_skip_seq
+end.
+
+
+ Ltac do_compute_expr1 Delta Pre e :=
+ match Pre with
+ | @exp _ _ ?A ?Pre1 => fail "BLA1"
+  (* let P := fresh "P" in let Q := fresh "Q" in let R := fresh "R" in
+  let H8 := fresh "DCE" in let H9 := fresh "DCE" in
+  evar (P: A -> list Prop);
+  evar (Q: A -> list localdef);
+  evar (R: A -> list mpred);
+  assert (H8: Pre1 =  (fun a => PROPx (P a) (LOCALx (Q a) (SEPx (R a)))))
+    by (extensionality; unfold P,Q,R; reflexivity);
+  let v := fresh "v" in evar (v: A -> val);
+  assert (H9: forall a, ENTAIL Delta, PROPx (P a) (LOCALx (Q a) (SEPx (R a))) |--
+                       local ((eq (v a)) (eval_expr e)))
+     by (let a := fresh "a" in intro a; do_compute_expr_helper Delta (Q a) v) *)
+
+ | PROPx ?P (LOCALx ?Q (SEPx ?R)) => fail "BLA2"
+
+ (* let H9 := fresh "H" in
+  let v := fresh "v" in (evar (v: val);
+  assert (H9:  ENTAIL Delta, PROPx P (LOCALx Q (SEPx R))|--
+                     local ((eq v) (eval_expr e)))
+   by (do_compute_expr_helper Delta Q v))  *)
+| _ => fail "YES"
+ end. 
+
+Ltac forward_switch' := 
+ match goal with
+| |- semax ?Delta (PROPx ?P (LOCALx ?Q (SEPx ?R))) (Sswitch ?e _) _ => 
+  let sign := constr:(signof e) in let sign := eval hnf in sign in
+   let HRE := fresh "H" in let v := fresh "v" in
+    evar (v: val);
+    do_compute_expr1 Delta P Q R e v HRE;
+    simpl in v;
+    let n := fresh "n" in evar (n: int); 
+    let H := fresh in assert (H: v=Vint n) by (unfold v,n; reflexivity);
+    let A := fresh in 
+    match goal with |- ?AA => set (A:=AA) end;
+    revert n H; normalize; intros n H; subst A;
+    let n' := fresh "n" in pose (n' := Int.unsigned n); 
+    let H' := fresh in assert (H': n = Int.repr n');
+    [try (symmetry; apply Int.repr_unsigned) 
+       | rewrite H,H' in HRE; clear H H';
+         subst n' n v; 
+         rewrite (Int.repr_unsigned (Int.repr _)) in HRE;
+          eapply semax_switch_PQR ; 
+           [reflexivity | check_typecheck | exact HRE 
+           | clear HRE; unfold select_switch at 1; unfold select_switch_default at 1;
+             try match goal with H := @abbreviate statement _ |- _ => clear H end;
+             process_cases sign ] 
+]
+
+end.
+
+Ltac forward_switch_seq post :=
+  check_Delta; check_POSTCONDITION;
+  repeat (apply -> seq_assoc; abbreviate_semax);
+  repeat apply -> semax_seq_skip;
+first [ignore (post: environ->mpred)
+      | fail 1 "Invariant (first argument to forward_if) must have type (environ->mpred)"];
+     match goal with
+     | _ : _ |- semax _ _ (Ssequence (Sswitch _ _) _) _ => 
+       apply semax_seq with post;
+       [forward_switch' 
+      | abbreviate_semax; 
+        simpl_ret_assert (*autorewrite with ret_assert*)]
+end.    
+
            match goal with
            | [ _ : _ |- semax _ ?Pre ?C ?Post ] =>
-             forward_switch Pre
-           end; clear Z0.
-           *** admit. (* (* RC_FAIL  *)             
+                forward_switch_seq Pre 
+            
+           end.
+
+ clear Z0. 
+           admit.
+           *** (* RC_FAIL  *)             
               match goal with
                  | [ _ : _ |- semax _ ?Pre ?C ?Post ] =>
                    forward_empty_while_break Pre
@@ -516,7 +754,7 @@ Proof.
              erewrite N.
              (* entailer!. *)
              admit. *)
-           *** admit. (* (* RC_FAIL: same *)
+       (*    *** admit. (* (* RC_FAIL: same *)
               match goal with
                  | [ _ : _ |- semax _ ?Pre ?C ?Post ] =>
                    forward_empty_while_break Pre
@@ -548,7 +786,7 @@ Proof.
              admit. *)
            *** admit. (* forward.
                entailer!. *) 
-           *** remember (map Vint (map Int.repr ptr)) as ptr'.
+           *** remember (map Vint ptr) as ptr'.
                normalize.
                Intros. 
                assert_PROP ((Vptr b i) = 
@@ -560,10 +798,10 @@ Proof.
                  econstructor;
                  auto.
                  repeat split; auto; 
-                   autorewrite with norm;  try rep_omega.
+                   autorewrite with norm;  try rep_lia.
                  cbn.
                  autorewrite with norm.
-                 rep_omega.
+                 rep_lia.
                  constructor.
                  intros.
                  econstructor; auto; cbn.
@@ -669,7 +907,7 @@ Proof.
                  res_v : Z, res_ptr : val *)   
                erewrite Heqptr'.
                replace (data_at Tsh (tarray tuchar (len ptr))
-                       (map Vint (map Int.repr ptr)) (Vptr b i))
+                       (map Vint ptr) (Vptr b i))
                        with
                         (data_at Tsh tuchar (Vubyte (Byte.repr (Znth 0 ptr)))
                                    (Vptr b i) * 
@@ -866,7 +1104,7 @@ Proof.
   temp _t'30 (Vint (Int.repr (len (tags td)))); 
   temp _t'15 Vzero; 
   temp _tlv_constr (Vint 0%int);
-  temp _t'13 Vzero; temp _t'34 (Znth 0 (map Vint (map Int.repr ptr)));
+  temp _t'13 Vzero; temp _t'34 (Znth 0 (map Vint ptr));
   temp _tag_len (Vint (Int.repr z0)); temp _t'35 (Vint (Int.repr (len (tags td))));
   temp _t'10 (Val.of_bool (Int.repr 0 == Int.repr (len (tags td)))%int);
   temp _tagno (Vint (Int.repr z)); temp _t'4 Vzero; 
@@ -1076,7 +1314,7 @@ Proof.
                repeat rewrite_if_b; symmetry; repeat Zbool_to_Prop;
                  try lia; auto. }
           erewrite B.
-          entailer!.
+          entailer!.  *)
 Admitted.
-*)
+
 End Ber_check_tags.
